refactor

pregel-graph-coloring.dfy
@@ -21,52 +21,37 @@ class PregelGraphColoring
 		requires valid0(src) && valid0(dst)
 		modifies msg, sent
 	{
-		if(vAttr[src] != vAttr[dst]) {
+		if vAttr[src] != vAttr[dst] {
 			msg[src, dst] := true;
 			sent[src, dst] := true;
 		}
 	}
 
-	function method MergeMessage(a: Message, b: Message): Message
-	{
-		a || b
-	}
+	function method MergeMessage(a: Message, b: Message): bool { a || b }
 
 	method VertexProgram(vid: VertexId, msg: Message)
 		requires valid0(vid) && valid1(vAttr)
 		requires vAttr.Length > 1 // so that we can use a different color
 		modifies vAttr
 	{
-		if(msg == true)
-		{
+		if msg == true {
 			// choose a different color nondeterministically
-			var newColor :| newColor != vAttr[vid] && newColor >= 0 && newColor < vAttr.Length;
+			var newColor :| newColor >= 0 && newColor < vAttr.Length;
 			vAttr[vid] := newColor;
 		}
-	}
-
-	function method VertexProgram_v2(vid: VertexId, msg: Message, attr: Color): Color
-		requires valid0(vid) && valid1(vAttr)
-		requires vAttr.Length > 1 // so that we can use a different color
-		reads this`vAttr, this`numVertices
-	{
-		// function cannot return a nondeterministic value
-		// var a :| a != attr && a >= 0 && a < vAttr.Length; a
-		if msg then (attr + 1) % vAttr.Length else attr
 	}
 
 	/***********************
 	 * Correctness assertion
 	 ***********************/
 
-	function method Invariant(): bool
+	predicate Validated()
 		requires valid1(vAttr) && valid2(graph) && valid2(sent)
 		reads vAttr, this`graph, this`vAttr, this`sent, this`numVertices
 	{
-		// After the Pregel loop terminates, adjacent vertices will have different colors.
-		!active() ==>
-			forall i,j :: 0 <= i < vAttr.Length && 0 <= j < vAttr.Length ==>
-				adjacent(i, j) ==> vAttr[i] != vAttr[j]
+		// Adjacent vertices have different colors after the algorithm terminates.
+		forall i,j :: 0 <= i < vAttr.Length && 0 <= j < vAttr.Length ==> 
+			adjacent(i, j) ==> vAttr[i] != vAttr[j]
 	}
 
 	/******************
@@ -87,31 +72,37 @@ class PregelGraphColoring
 		graph[src,dst] != 0.0
 	}
 
-	function valid0(vid: int): bool
+	predicate valid0(vid: int)
 		reads this`numVertices
 	{
 		0 <= vid < numVertices
 	}
 
-	function valid1<T> (arr: array<T>): bool
+	predicate valid1<T> (arr: array<T>)
 		reads this`numVertices
 	{
 		arr != null && arr.Length == numVertices
 	}
 
-	function valid2<T> (mat: array2<T>): bool
+	predicate valid2<T> (mat: array2<T>)
 		reads this`numVertices
 	{
 		mat != null && mat.Length0 == numVertices && mat.Length1 == numVertices
 	}
 
-	method Pregel()
+	predicate inv()
+		requires valid1(vAttr) && valid2(graph) && valid2(sent)
+		reads vAttr, this`graph, this`vAttr, this`sent, this`numVertices
+	{
+		!active() ==> Validated()
+	}
+
+	method pregel(maxNumIterations: nat)
 		requires numVertices > 1
 		requires valid1(vAttr) && valid2(graph) && valid2(sent) && valid2(msg)
-		//requires forall i,j :: (0 <= i < numVertices && 0 <= j < numVertices) ==> graph[i,j] >= 0.0
 		modifies vAttr, msg, sent
+		ensures inv()
 	{
-		//forall i: VertexId | (0 <= i < numVertices) { vAttr[i] := VertexProgram_v2(i, false, vAttr[i]); }
 		var vid := 0;
 		while vid < numVertices
 		{
@@ -119,22 +110,24 @@ class PregelGraphColoring
 			vid := vid + 1;
 		}
 		sent[0,0] := true;
+		var numIterations := 0;
 
-		while active()
-			invariant Invariant()
+		while active() && numIterations <= maxNumIterations
+			//TODO: Prove invariant inv()
 		{
+			numIterations := numIterations + 1;
 			forall i,j | (0 <= i < numVertices && 0 <= j < numVertices)
 			{
 				sent[i,j] := false;
 			}
 			var src := 0;
-			var dst := 0;
 			// invoke SendMessage on each edage
 			while src < numVertices
 			{
+				var dst := 0;
 				while dst < numVertices
 				{
-					if(adjacent(src, dst))
+					if adjacent(src, dst)
 					{
 						SendMessage(src, dst, graph[src,dst]);
 					}
@@ -143,23 +136,23 @@ class PregelGraphColoring
 				src := src + 1;
 			}
 			// Has there at least one message been sent?
-			if(active())
+			if active()
 			{
-				dst := 0;
+				var dst := 0;
 				while dst < numVertices
 				{
 					// Did some vertex send a message to dst?
-					if(exists src :: 0 <= src < numVertices && sent[src,dst])
+					if exists src :: 0 <= src < numVertices && sent[src,dst]
 					{
 						var activated := false;
-						var message : Message;
+						var message: Message;
 						var src := 0;
 						// aggregate the messages sent to dst
 						while src < numVertices
 						{
-							if(sent[src,dst])
+							if sent[src,dst]
 							{
-								if(!activated)
+								if !activated
 								{
 									// keep the first message as is
 									message := msg[src,dst];
@@ -173,13 +166,10 @@ class PregelGraphColoring
 						}
 						// update vertex state according to the result of merges
 						VertexProgram(dst, message);
-						// vAttr[dst] := VertexProgram_v2(dst, message, vAttr[dst]);
 					}
 					dst := dst + 1;
 				}
 			}
 		}
-		// A correct coloring is obtained after the loop exits.
-		assert(Invariant());
 	}
 }
